F*/fun/Tactic.fst
@@ -1,0 +1,29 @@
+module Tactic
+
+open FStar.Tactics
+open FStar.List
+
+val ex1 : unit -> Lemma True
+let ex1 () =
+    assert_by_tactic True (fun () -> ())
+
+val ex2 : unit -> Lemma True
+let ex2 () =
+    assert_by_tactic True (fun () -> (dump "Example 3"))
+
+let tau3 () : Tac unit =
+  dump "before split";
+  Tactics.split ();
+  dump "After split";
+  // comment out smt and the next poor will fail
+  smt ();
+  trivial ()
+
+val ex3 : x : nat → Lemma (x + x >= 0 /\ List.length [4;5;1] == 3)
+let ex3 (x : nat) =
+  assert_by_tactic (x + x >= 0 /\ List.length [4;5;1] == 3) tau3
+
+(* but first a helper *)
+
+let test_tactic () : Tac unit =
+  dump "first"
